Software/Doc/Example/Verification/System1/Package/NatRangeIterator.v
@@ -10,6 +10,79 @@ Import ObjectOrientedNotations.
 Open Scope oo_scope.
 Open Scope exec_scope.
 
+Notation "ref '/' st1 '-->' st2" := (transition exec_step ref st1 st2)
+  (at level 40, st1 at level 39, format "'[' ref  /  st1  '-->'  st2 ']'").
+
+Notation "ref '/' st1 '-->+' st2" := (clos_refl_trans_1n state (transition exec_step ref) st1 st2)
+  (at level 40, st1 at level 39, format "'[' ref  /  st1  '-->+'  st2 ']'").
+
+Notation "ref '/' st1 '-->*' st2" := (clos_refl_trans_term state (transition exec_step ref) st1 st2)
+  (at level 40, st1 at level 39, format "'[' ref  /  st1  '-->*'  st2 ']'").
+
+Definition a : term := tref 1.
+Definition config_state : state :=
+Cstate
+  (nil :: nil)%list
+  (nil :: nil)%list
+  (tvoid :: tcl "NatRangeIterator" <(tbool true, tnat 3, tnat 2)> :: nil)%list
+.
+
+Lemma config_state_valid :
+  (tnat 2 # "NatRangeIterator_make"|(tnat 3)|) / init_state ==>* a / config_state.
+Proof.
+  unfold a, config_state.
+  repeat reduce.
+  eapply Relation_Operators.rt1n_refl.
+  Qed.
+
+Ltac invert_termination :=
+  match goal with
+  | H: clos_refl_trans_term exec_state exec_step ?x ?y1, H0: clos_refl_trans_term exec_state exec_step ?x ?y2 |- _ =>
+    assert (y2 = y1);
+    [apply (clos_refl_trans_term_is_function exec_state exec_step is_function_exec_step x y1 y2 H H0) |]
+  end.
+
+Lemma all_states_wf_config_state :
+  all_states_wf exec_step a config_state.
+Proof.
+  unfold all_states_wf. intros.
+  remember config_state as x eqn:Hx.
+  induction H; intros; subst x.
+  - unfold wf, config_state.
+    exists 1. exists true. exists 3. exists 2.
+    unfold wf_fun. simpl. repeat split; try solve [reflexivity].
+    intros Hcontra. inversion Hcontra.
+  - induction H.
+    + assert (a # "off"|()| / config_state ==>* tbool true / config_state).
+      { unfold a, config_state. repeat reduce. apply Relation_Operators.rt1n_refl. }
+      invert_termination. inversion H2. subst result y. clear H1 H2.
+      apply IHclos_refl_trans_1n. reflexivity.
+    + assert (a # "after"|()| / config_state ==>* tbool false / config_state).
+      { unfold a, config_state. repeat reduce. apply Relation_Operators.rt1n_refl. }
+      invert_termination. inversion H2. subst result y. clear H1 H2.
+      apply IHclos_refl_trans_1n. reflexivity.
+    + remember (Cstate (nil :: nil)%list (nil :: nil)%list (tvoid :: tcl "NatRangeIterator" <(tbool false, tnat 3, tnat 2)> :: nil)%list)
+        as st2.
+      assert (a # "forth"|()| / config_state ==>* tvoid / st2).
+      { rewrite Heqst2. unfold a, config_state. repeat reduce. apply Relation_Operators.rt1n_refl. }
+      invert_termination. inversion H3. subst result y. clear H2 H3.
+
+(**
+
+We can proceed in one of two ways:
+
+- Explore all reachable states by calling 'forth' until we are 'after', and show that
+  each state reached is well-formed.
+- Create an induction principle on 'forth' that somehow gets us out of explicit state
+  search. Basically we have to prove that calling forth results in a well formed state, based ONLY
+  on the assumption that the current state is well-formed.
+
+Ultimately, we come upon the problem of proof again: in order to prove something without
+resorting to enumerating all reachable states, we must have an induction principle.
+
+*)
+  Abort.
+
 Lemma proof_get_at_start :
   get_at_start exec_step.
 Proof.
